chore: slug cleanup

src/verso-manual/Verso/Genre/Manual/Slug.lean
@@ -3,23 +3,72 @@ Copyright (c) 2023-2024 Lean FRO LLC. All rights reserved.
 Released under Apache 2.0 license as described in the file LICENSE.
 Author: David Thrane Christiansen
 -/
-
+import Std.Data.HashSet
 import Verso.Method
 
 namespace Verso.Genre.Manual
 open Verso.Method
 open Lean (ToJson FromJson)
+open Std (HashSet)
+
+def Slug.validChars := "abcdefghijklmnopqrstuvwxyzABCDEFGHIJKLMNOPQRSTUVWXYZ0123456789-".toList
+
+
+def asSlug (str : String) : String :=
+  let rec loop (iter : String.Iterator) (acc : String) : String :=
+    if iter.atEnd then acc
+    else
+      let c := iter.curr
+      loop iter.next <|
+        if c ∈ Slug.validChars then acc.push c
+        else acc
+  loop str.iter ""
+
+def Slug.WF (str : String) : Prop := ∀ c, c ∈ str.data → c ∈ validChars
+
+theorem Slug.wf_push : c ∈ validChars → WF str → WF (str.push c) := by
+  unfold WF
+  intro _ wf _ mem
+  simp only [String.data_push, List.mem_append, List.mem_singleton] at mem
+  cases mem
+  . apply wf; assumption
+  . simp [*]
+
+theorem Slug.asSlug_loop_valid : WF acc → WF (asSlug.loop iter acc) := by
+  intro wfAcc
+  induction iter, acc using asSlug.loop.induct <;> unfold asSlug.loop <;> simp [*]
+  case case2 iter acc notEnd c ih =>
+    apply ih
+    unfold WF
+    intro c'
+    unfold WF at wfAcc
+    split
+    . simp; intro h; cases h
+      . apply wfAcc; assumption
+      . simp [*]
+    . apply wfAcc
+
+theorem Slug.asSlug_valid : WF (asSlug str) := by
+  unfold asSlug
+  apply asSlug_loop_valid
+  unfold WF; intro c h; cases h
 
 structure Slug where
   private mk ::
   toString : String
+  wf : Slug.WF toString
 deriving BEq, Hashable, DecidableEq, Ord, Repr
 
+instance : ToString Slug := ⟨Slug.toString⟩
+
 instance : ToJson Slug where
-  toJson | ⟨str⟩ => ToJson.toJson str
+  toJson | ⟨str, _⟩ => ToJson.toJson str
 
 instance : FromJson Slug where
-  fromJson? v := Slug.mk <$> FromJson.fromJson? v
+  fromJson? v := do
+    let s : String ← FromJson.fromJson? v
+    if h : asSlug s = s then pure ⟨s, h ▸ Slug.asSlug_valid⟩
+    else throw s!"String {s} contains invalid characters"
 
 namespace Slug
 
@@ -37,27 +86,16 @@ instance : DecidableRel (@LE.le Slug _) := fun s1 s2 =>
   else if h' : s1.toString < s2.toString then .isTrue (.inr h')
   else .isFalse <| by intro nope; cases nope <;> contradiction
 
-instance : Coe String Slug where
-  coe := (⟨·⟩)
-
-defmethod String.sluggify (str : String) : Slug := Id.run do
-  let mut s := ""
-  for c in str.data do
-    if c.isAlpha then
-      s := s.push c.toLower
-    else if c.isDigit then
-      s := s.push c
-    else if c == ' ' || c == '-' then
-      s := s.push '-'
-  ⟨s⟩
+defmethod String.sluggify (str : String) : Slug :=
+  ⟨asSlug str, asSlug_valid⟩
 
 def ofString (str : String) : Slug := str.sluggify
 
-partial def unique (used : Lean.HashSet Slug) (slug : Slug) : Slug :=
+partial def unique (used : HashSet Slug) (slug : Slug) : Slug :=
   if !(used.contains slug) then slug
   else
     let rec attempt (i : Nat) :=
-      let slug' := s!"{slug.toString}{i}"
+      let slug' := s!"{slug.toString}{i}".sluggify
       if !(used.contains slug') then slug'
       else attempt (i + 1)
     attempt 1
